theories/base.v
@@ -6,9 +6,3 @@ From iris.bi Require Export
   lib.fractional.
 From iris.base_logic Require Export
   lib.invariants.
-
-From caml5 Require Import
-  prelude.
-
-Definition caml5_namespace :=
-  nroot .@ "caml5".
