theories/std/base.v
@@ -4,6 +4,3 @@ From caml5.program_logic Require Export
   atomic.
 From caml5.lang Require Export
   lang.
-
-Definition std_namespace :=
-  caml5_namespace .@ "std".
